dh.v
@@ -23,59 +23,21 @@ Implicit Types kA kB : term.
 
 Variable P : term → iProp.
 
-Definition dh_pred t : iProp :=
-  ∃ g a, ⌜t = TExp g [TNonce a]⌝ ∧ □ P (TNonce a).
-
-Definition dh_nonce a : iProp := nonce_pred a dh_pred.
-
-Fact dh_gen_key : unit. Proof. exact: tt. Qed.
-
-Definition dh_gen g : iProp :=
-  locked_with dh_gen_key (
-    ∀ ts, [∗ set] a ∈ nonces_of_term g, published a (TExp g ts))%I.
-
-Canonical dh_gen_unlockable g := [unlockable of dh_gen g].
-
-Global Instance Persistent_dh_gen g : Persistent (dh_gen g).
-Proof. rewrite unlock; apply _. Qed.
-
-Lemma dh_gen_sterm g : dh_gen g -∗ sterm g.
-Proof.
-rewrite unlock; iIntros "H"; iSpecialize ("H" $! []).
-rewrite [in sterm _]unlock.
-iApply (big_sepS_mono with "H") => ??.
-iApply published_declared_nonce.
-Qed.
-
-Lemma nonces_of_term_dh_gen g :
-  nonces_of_term g = ∅ →
-  ⊢ dh_gen g.
-Proof.
-rewrite unlock => ->.
-by iIntros (ts); rewrite big_sepS_empty.
-Qed.
+Definition dh_publ t : iProp :=
+  ∃ g a, ⌜t = TExp g [a]⌝ ∧ □ P a.
 
 Definition dh_seed t : iProp :=
-  match t with
-  | TNonce a => dh_nonce a
-  | _ => False
-  end.
-
-Global Instance Persistent_dh_seed t : Persistent (dh_seed t).
-Proof. case: t =>>; apply _. Qed.
+  sterm t ∧
+  □ (pterm t ↔ ▷ False) ∧
+  □ (∀ t', dh_pred t t' ↔ ▷ □ dh_publ t').
 
 Lemma dh_seed_elim0 a :
   dh_seed a -∗
   pterm a -∗
   ▷ False.
 Proof.
-iIntros "#aP #p_t".
-case: a => //= a.
-rewrite pterm_TNonce.
-iPoseProof (publishedE with "aP p_t") as "{p_t} p_t".
-iIntros "!>".
-iDestruct "p_t" as (g' a') "# [%e p_t]".
-by move/(f_equal is_exp): e; rewrite is_exp_TExp.
+iIntros "#(_ & aP & _) #p_t".
+by iApply "aP".
 Qed.
 
 Lemma dh_seed_elim1 g a :
@@ -84,14 +46,12 @@ Lemma dh_seed_elim1 g a :
   ▷ P a.
 Proof.
 iIntros "#aP #p_t".
-rewrite pterm_TExp1 big_sepS_union_pers.
-iDestruct "p_t" as "[[? contra]|[_ p_t]]".
+rewrite pterm_TExp1.
+iDestruct "p_t" as "(_ & _ & [contra | p_t])".
   by iPoseProof (@dh_seed_elim0 with "aP contra") as ">[]".
-case: a => //= a.
-rewrite nonces_of_term_eq /= big_sepS_singleton.
-iPoseProof (publishedE with "aP p_t") as "{p_t} p_t".
-iIntros "!>".
-iDestruct "p_t" as (g' a') "# [%e p_t]".
+iDestruct "aP" as "(_ & _ & #aP)".
+iSpecialize ("aP" with "p_t"); iModIntro.
+iDestruct "aP" as (g' a') "# [%e aP]".
 by case/TExp_inj: e => _ /Permutation_singleton [] ->; eauto.
 Qed.
 
@@ -101,13 +61,12 @@ Lemma dh_seed_elim2 g a t :
   ◇ (pterm (TExp g [a]) ∧ pterm t).
 Proof.
 iIntros "#aP #p_t".
-rewrite pterm_TExp2 !big_sepS_union_pers.
-iDestruct "p_t" as "[[??] | [[? contra] | p_t]]"; eauto.
-  by iPoseProof (dh_seed_elim0 with "aP contra") as ">[]".
-case: a => //= a.
-iDestruct "p_t" as "([_ p_t] & _)".
-rewrite nonces_of_term_eq /= big_sepS_singleton.
-iPoseProof (publishedE with "aP p_t") as "{p_t} p_t".
+rewrite pterm_TExp2.
+iDestruct "p_t" as "[p_t|[[_ contra]|p_t]]"; eauto.
+  by iPoseProof (@dh_seed_elim0 with "aP contra") as ">[]".
+iDestruct "p_t" as "(_ & p_t & _)".
+iDestruct "aP" as "(_ & _ & #aP)".
+iPoseProof ("aP" with "p_t") as "{p_t} p_t".
 iAssert (▷ False)%I as ">[]".
 iModIntro.
 iDestruct "p_t" as (g' a') "(%e & _)".
@@ -115,18 +74,14 @@ by case/TExp_inj: e => _ /Permutation_length.
 Qed.
 
 Lemma dh_pterm_TExp g a :
-  dh_gen g -∗
+  sterm g -∗
   dh_seed a -∗
   ▷ □ P a -∗
   pterm (TExp g [a]).
 Proof.
-rewrite unlock; iIntros "#gP #aP #P_a".
-rewrite pterm_TExp1; iRight.
-case: a => //= a.
-rewrite big_sepS_union_pers; iSplit; first by iApply "gP".
-rewrite nonces_of_term_eq /= big_sepS_singleton.
-iExists _; iSplit; eauto.
-by iExists g, a; eauto.
+iIntros "#gP #(? & ? & aP) #P_a".
+rewrite pterm_TExp1; do !iSplit => //.
+by iRight; iApply "aP"; iModIntro; iExists _, _; eauto.
 Qed.
 
 Definition mkdh : val := mknonce.
@@ -134,14 +89,15 @@ Definition mkdh : val := mknonce.
 Lemma wp_mkdh E (Ψ : val → iProp) :
   (∀ a, sterm a -∗
         dh_seed a -∗
-        crypto_meta_token a (⊤ ∖ ↑cryptoN.@"nonce") -∗ Ψ a) -∗
+        term_meta_token a ⊤ -∗ Ψ a) -∗
   WP mkdh #() @ E {{ Ψ }}.
 Proof.
-iIntros "post"; iApply (wp_mknonce _ (dh_pred)).
-iIntros (a) "#s_a #aP token"; iApply "post" => //.
-rewrite /crypto_meta_token nonces_of_term_eq /=.
-iSplit; first by iPureIntro; set_solver.
-by rewrite big_sepS_singleton.
+iIntros "post"; iApply (wp_mknonce _ False%I dh_publ).
+iIntros (a) "#s_a #(aP1 & aP2) #? token"; iApply "post" => //.
+do !iSplit => //.
+iModIntro; iSplit.
+- by iIntros "H"; iSpecialize ("aP1" with "H"); iModIntro.
+- by iIntros "#?"; iApply "aP2"; iModIntro.
 Qed.
 
 End DH.
